txn-data-consistency/EP+_TCCv_Draft.thy
@@ -1,4 +1,4 @@
-theory "EP+_TCCv_update_kv_invs"
+theory "EP+_TCCv_Draft"
   imports "EP+_TCCv_proof"
 begin
 
